@prefix : <http://purl.org/cbv#> .
@prefix dc: <http://purl.org/dc/elements/1.1/> .
@prefix owl: <http://www.w3.org/2002/07/owl#> .
@prefix rdf: <http://www.w3.org/1999/02/22-rdf-syntax-ns#> .
@prefix xml: <http://www.w3.org/XML/1998/namespace> .
@prefix xsd: <http://www.w3.org/2001/XMLSchema#> .
@prefix rdfs: <http://www.w3.org/2000/01/rdf-schema#> .
@base <http://purl.org/cbv> .

<http://purl.org/cbv> rdf:type owl:Ontology ;
                      
                      owl:imports <http://protege.stanford.edu/plugins/owl/dc/protege-dc.owl> .


#################################################################
#
#    Annotation properties
#
#################################################################


dc:creator dc:creator "Monika Solanki(m.solanki@aston.ac.uk)" .



owl:versionInfo owl:versionInfo "1.1" .



rdfs:comment rdf:type owl:AnnotationProperty ;
             
             rdfs:comment "The CBVVocab is an OWL ontology that captures the identifiers in CBV 1.0 specification. (http://www.gs1.org/gsmp/kc/epcglobal/cbv/cbv_1_0-standard-20101013.pdf). The current version, CBVVocab 1.1, includes a partial set of the new identifiers to be included in CBV 1.1" .



dc:title dc:title "CBVVocab 1.1" .





#################################################################
#
#    Datatypes
#
#################################################################


###  http://www.w3.org/1999/02/22-rdf-syntax-ns#PlainLiteral

rdf:PlainLiteral rdf:type rdfs:Datatype .



###  http://www.w3.org/2000/01/rdf-schema#Literal

rdfs:Literal rdf:type rdfs:Datatype .



###  http://www.w3.org/2001/XMLSchema#anyURI

xsd:anyURI rdf:type rdfs:Datatype .



###  http://www.w3.org/2001/XMLSchema#positiveInteger

xsd:positiveInteger rdf:type rdfs:Datatype .



###  http://www.w3.org/2001/XMLSchema#string

xsd:string rdf:type rdfs:Datatype .





#################################################################
#
#    Object Properties
#
#################################################################


###  http://purl.org/cbv#hasSite

:hasSite rdf:type owl:ObjectProperty ;
         
         owl:inverseOf :hasSubSite .



###  http://purl.org/cbv#hasSubSite

:hasSubSite rdf:type owl:ObjectProperty ;
            
            rdfs:domain :Site ;
            
            rdfs:range :SubSite .



###  http://purl.org/cbv#hasSubSiteAttribute

:hasSubSiteAttribute rdf:type owl:ObjectProperty .



###  http://purl.org/cbv#hasSubSiteType

:hasSubSiteType rdf:type owl:ObjectProperty .





#################################################################
#
#    Data properties
#
#################################################################


###  http://purl.org/cbv#hasLocationID

:hasLocationID rdf:type owl:DatatypeProperty ;
               
               rdfs:domain :Site ;
               
               rdfs:range xsd:string .



###  http://purl.org/cbv#hasNumericalCode

:hasNumericalCode rdf:type owl:DatatypeProperty ,
                           owl:FunctionalProperty ;
                  
                  rdfs:domain :SubSiteType ;
                  
                  rdfs:range xsd:positiveInteger .



###  http://purl.org/cbv#hasSubSiteDetail

:hasSubSiteDetail rdf:type owl:DatatypeProperty ;
                  
                  owl:equivalentProperty :ssd .



###  http://purl.org/cbv#ssd

:ssd rdf:type owl:DatatypeProperty .





#################################################################
#
#    Classes
#
#################################################################


###  http://purl.org/cbv#BusinessStep

:BusinessStep rdf:type owl:Class ;
              
              rdfs:comment """ Denotes a specific activity within a business process. The business step field of an event specifies what business process step was taking place that caused the event to be captured. Example: an EPCIS event is generated as a product departs the location
identified by the Read Point. Business Step = <The identifier that denotes“shipping”>
""" .



###  http://purl.org/cbv#Disposition

:Disposition rdf:type owl:Class ;
             
             rdfs:comment """ Denotes the business state of an object. The disposition field of anevent specifies the business condition of the subject of the event (the things specified in the“what”
dimension), subsequent to the event. The disposition is assumed to hold true until another event indicates a change of disposition.  Example: an EPCIS event is generated and afterward the products can be sold as-is and customers can access product for purchase. Disposition = <The identifier that denotes“sellable and accessible”> """ .



###  http://purl.org/cbv#Site

:Site rdf:type owl:Class ;
      
      owl:equivalentClass [ rdf:type owl:Restriction ;
                            owl:onProperty :hasLocationID ;
                            owl:qualifiedCardinality "1"^^xsd:nonNegativeInteger ;
                            owl:onDataRange xsd:string
                          ] .



###  http://purl.org/cbv#SourceDestinationType

:SourceDestinationType rdf:type owl:Class .



###  http://purl.org/cbv#SubSite

:SubSite rdf:type owl:Class ;
         
         owl:equivalentClass [ rdf:type owl:Class ;
                               owl:intersectionOf ( [ rdf:type owl:Restriction ;
                                                      owl:onProperty :hasSite ;
                                                      owl:someValuesFrom :Site
                                                    ]
                                                    [ rdf:type owl:Restriction ;
                                                      owl:onProperty :hasSubSiteType ;
                                                      owl:someValuesFrom :SubSiteType
                                                    ]
                                                  )
                             ] ;
         
         rdfs:subClassOf [ rdf:type owl:Restriction ;
                           owl:onProperty :hasSubSiteAttribute ;
                           owl:allValuesFrom :SubSiteAttribute
                         ] ,
                         [ rdf:type owl:Restriction ;
                           owl:onProperty :hasSubSiteDetail ;
                           owl:minCardinality "0"^^xsd:nonNegativeInteger
                         ] ,
                         [ rdf:type owl:Restriction ;
                           owl:onProperty :hasSubSiteAttribute ;
                           owl:minCardinality "0"^^xsd:nonNegativeInteger
                         ] .



###  http://purl.org/cbv#SubSiteAttribute

:SubSiteAttribute rdf:type owl:Class .



###  http://purl.org/cbv#SubSiteType

:SubSiteType rdf:type owl:Class .



###  http://purl.org/cbv#TransactionType

:TransactionType rdf:type owl:Class ;
                 
                 rdfs:comment " Denotes a particular kind of business transaction. Example: the identifier that denotes “purchase order”. " .



###  http://www.w3.org/2002/07/owl#Thing

owl:Thing rdf:type owl:Class .





#################################################################
#
#    Individuals
#
#################################################################


###  http://purl.org/cbv#BackRoom

:BackRoom rdf:type :SubSiteType ,
                   owl:NamedIndividual ;
          
          :hasNumericalCode "201"^^xsd:positiveInteger ;
          
          rdfs:comment """An area within a store (all formats - club, etc) used to hold
product until it is purchased or can be moved to the sales floor""" .



###  http://purl.org/cbv#CargoTerminal

:CargoTerminal rdf:type :SubSiteType ,
                        owl:NamedIndividual ;
               
               :hasNumericalCode "215"^^xsd:positiveInteger ;
               
               rdfs:comment "An area where cargo may get transferred between carriers." .



###  http://purl.org/cbv#ColdStorage

:ColdStorage rdf:type :SubSiteAttribute ,
                      owl:NamedIndividual ;
             
             :hasNumericalCode "402"^^xsd:positiveInteger ;
             
             rdfs:comment """A specific area or room that maintains a temperature above
freezing but below ambient room temperature""" .



###  http://purl.org/cbv#ContainerDeck

:ContainerDeck rdf:type :SubSiteType ,
                        owl:NamedIndividual ;
               
               :hasNumericalCode "214"^^xsd:positiveInteger ;
               
               rdfs:comment "An area on board a shipping vessel where containers are loaded." .



###  http://purl.org/cbv#CustomerPickUpArea

:CustomerPickUpArea rdf:type :SubSiteType ,
                             owl:NamedIndividual ;
                    
                    :hasNumericalCode "212"^^xsd:positiveInteger ;
                    
                    rdfs:comment """An area designated at a store for customer to take possession of
purchased product.""" .



###  http://purl.org/cbv#Electronics

:Electronics rdf:type :SubSiteAttribute ,
                      owl:NamedIndividual ;
             
             :hasNumericalCode "401"^^xsd:positiveInteger ;
             
             rdfs:comment """A specific area within the store for holding electronic products
such as TV's, DVD players, etc.""" .



###  http://purl.org/cbv#Frozen

:Frozen rdf:type :SubSiteAttribute ,
                 owl:NamedIndividual ;
        
        :hasNumericalCode "402"^^xsd:positiveInteger ;
        
        rdfs:comment """A specific area or room that maintains a temperature at or below
freezing""" .



###  http://purl.org/cbv#PackagingArea

:PackagingArea rdf:type :SubSiteType ,
                        owl:NamedIndividual ;
               
               :hasNumericalCode "251"^^xsd:positiveInteger ;
               
               rdfs:comment "An area within a facility where product is packaged." .



###  http://purl.org/cbv#PharmacyArea

:PharmacyArea rdf:type :SubSiteType ,
                       owl:NamedIndividual ;
              
              :hasNumericalCode "253"^^xsd:positiveInteger .



###  http://purl.org/cbv#PickingArea

:PickingArea rdf:type :SubSiteType ,
                      owl:NamedIndividual ;
             
             :hasNumericalCode "252"^^xsd:positiveInteger ;
             
             rdfs:comment """An area within a facility in which product is picked to fulfill an
order.""" .



###  http://purl.org/cbv#ProductionArea

:ProductionArea rdf:type :SubSiteType ,
                         owl:NamedIndividual ;
                
                :hasNumericalCode "208"^^xsd:positiveInteger ;
                
                rdfs:comment """An area within a facility where the conversion of materials and
or assembly of components to manufacture goods, products or
services takes place.""" .



###  http://purl.org/cbv#ReceivingArea

:ReceivingArea rdf:type :SubSiteType ,
                        owl:NamedIndividual ;
               
               :hasNumericalCode "209"^^xsd:positiveInteger ;
               
               rdfs:comment """An area within a facility where incoming merchandise is
unloaded and checked for condition and completeness""" .



###  http://purl.org/cbv#ReturnsArea

:ReturnsArea rdf:type :SubSiteType ,
                      owl:NamedIndividual ;
             
             :hasNumericalCode "207"^^xsd:positiveInteger ;
             
             rdfs:comment """An area within a facility for holding or consolidating product to
be sent back to the supplier, shipper or designated location""" .



###  http://purl.org/cbv#SalesFloor

:SalesFloor rdf:type :SubSiteType ,
                     owl:NamedIndividual ;
            
            :hasNumericalCode "203"^^xsd:positiveInteger ;
            
            rdfs:comment """An area within a store (all formats - club, etc) where product is
displayed for customer purchase""" .



###  http://purl.org/cbv#SalesFloorTransitionArea

:SalesFloorTransitionArea rdf:type :SubSiteType ,
                                   owl:NamedIndividual ;
                          
                          :hasNumericalCode "211"^^xsd:positiveInteger ;
                          
                          rdfs:comment """An area within a store between two physical locations (e.g.
Backroom and Sales Floor) - used for a read point only""" .



###  http://purl.org/cbv#Shelf

:Shelf rdf:type :SubSiteAttribute ,
                owl:NamedIndividual ;
       
       :hasNumericalCode "403"^^xsd:positiveInteger ;
       
       rdfs:comment "A specified internal location for holding product." .



###  http://purl.org/cbv#ShippingArea

:ShippingArea rdf:type :SubSiteType ,
                       owl:NamedIndividual ;
              
              :hasNumericalCode "210"^^xsd:positiveInteger ;
              
              rdfs:comment """An area within a facility where outgoing merchandise is
checked for condition and completeness and loaded onto a
conveyance for transport""" .



###  http://purl.org/cbv#StorageArea

:StorageArea rdf:type :SubSiteType ,
                      owl:NamedIndividual ;
             
             :hasNumericalCode "202"^^xsd:positiveInteger ;
             
             rdfs:comment """An area where product is kept within a facility to fulfill future
need.""" .



###  http://purl.org/cbv#Undefined

:Undefined rdf:type :SubSiteType ,
                    owl:NamedIndividual ;
           
           :hasNumericalCode "299"^^xsd:positiveInteger ;
           
           rdfs:comment "Any sub-site type not identified by any of the listed values" .



###  http://purl.org/cbv#Yard

:Yard rdf:type :SubSiteType ,
               owl:NamedIndividual ;
      
      :hasNumericalCode "213"^^xsd:positiveInteger ;
      
      rdfs:comment """An area outside of the main building used for holding product
(e.g. Trailer or container)""" .



###  http://purl.org/cbv#accepting

:accepting rdf:type :BusinessStep ,
                    owl:NamedIndividual ;
           
           rdfs:comment """Denotes a specific activity within a business process where an object (i.e. product, shipment or asset) arrives into a location causing a change of 
        possession and/or responsibility.""" .



###  http://purl.org/cbv#active

:active rdf:type :Disposition ,
                 owl:NamedIndividual .



###  http://purl.org/cbv#arriving

:arriving rdf:type :BusinessStep ,
                   owl:NamedIndividual ;
          
          rdfs:comment "Shipment is arriving at a location" .



###  http://purl.org/cbv#assembling

:assembling rdf:type :BusinessStep ,
                     owl:NamedIndividual ;
            
            rdfs:comment """Denotes an activity within a business process whereby one or more trade item(s) or
        identifiable component parts are combined with other objects creating a new
        finished product. """ .



###  http://purl.org/cbv#bol

:bol rdf:type :TransactionType ,
              owl:NamedIndividual .



###  http://purl.org/cbv#collecting

:collecting rdf:type :BusinessStep ,
                     owl:NamedIndividual ;
            
            rdfs:comment """ Denotes a specific activity within a business process where an object (i.e.
        product, asset, shipment or container) is picked up and collected for future
        disposal, recycling or reused. """ .



###  http://purl.org/cbv#commissioning

:commissioning rdf:type :BusinessStep ,
                        owl:NamedIndividual ;
               
               rdfs:comment """   Process of associating an EPC with a particular object (product, shipment, asset
        or container). A tag may have been encoded and applied in this step, or may have
        been previously encoded.  """ .



###  http://purl.org/cbv#consigning

:consigning rdf:type :BusinessStep ,
                     owl:NamedIndividual ;
            
            rdfs:comment """Added in CBV 1.1. Indicates the overall process of staging_outbound, loading, departing, and accepting. 
It may be used when more granular process step
information is unknown or inaccessible. The use of consigning is
mutually exclusive from the use of staging_outbound, loading, departing, and accepting. 
Note: This business step is similar to shipping, but includes a change of possession and/or
ownership at the outbound side""" .



###  http://purl.org/cbv#container__closed

:container__closed rdf:type :Disposition ,
                            owl:NamedIndividual .



###  http://purl.org/cbv#cycle_counting

:cycle_counting rdf:type :BusinessStep ,
                         owl:NamedIndividual ;
                
                rdfs:comment "Added in version 1.1" .



###  http://purl.org/cbv#decommissioning

:decommissioning rdf:type :BusinessStep ,
                          owl:NamedIndividual ;
                 
                 rdfs:comment """ Process of disassociating an EPC with an object (i.e. product, shipment, asset or container). EPC may
be re-commissioned at some point in the future and read again – however only with new
information. """ .



###  http://purl.org/cbv#departing

:departing rdf:type :BusinessStep ,
                    owl:NamedIndividual ;
           
           rdfs:comment "   Shipment is leaving a location on its way to a destination " .



###  http://purl.org/cbv#desadv

:desadv rdf:type :TransactionType ,
                 owl:NamedIndividual .



###  http://purl.org/cbv#destroyed

:destroyed rdf:type :Disposition ,
                    owl:NamedIndividual .



###  http://purl.org/cbv#destroying

:destroying rdf:type :BusinessStep ,
                     owl:NamedIndividual ;
            
            rdfs:comment """ Process of terminating an object (i.e. product, shipment, asset or shipping
        container) The object and its EPC should not be the subject of subsequent events
        that require a physical observation; subsequent physical observations are likely
        indicative of error (such as a stray read of a tag inside an incinerator)  """ .



###  http://purl.org/cbv#disassembling

:disassembling rdf:type :BusinessStep ,
                        owl:NamedIndividual ;
               
               rdfs:comment """      Denotes a specific activity within a business process where a trade item is broken
        down into separate, uniquely identified component parts.  """ .



###  http://purl.org/cbv#encoded

:encoded rdf:type :Disposition ,
                  owl:NamedIndividual .



###  http://purl.org/cbv#encoding

:encoding rdf:type :BusinessStep ,
                   owl:NamedIndividual .



###  http://purl.org/cbv#entering_exiting

:entering_exiting rdf:type :BusinessStep ,
                           owl:NamedIndividual .



###  http://purl.org/cbv#holding

:holding rdf:type :BusinessStep ,
                  owl:NamedIndividual .



###  http://purl.org/cbv#in_progress

:in_progress rdf:type :Disposition ,
                      owl:NamedIndividual .



###  http://purl.org/cbv#in_transit

:in_transit rdf:type :Disposition ,
                     owl:NamedIndividual .



###  http://purl.org/cbv#inactive

:inactive rdf:type :Disposition ,
                   owl:NamedIndividual .



###  http://purl.org/cbv#inspecting

:inspecting rdf:type :BusinessStep ,
                     owl:NamedIndividual .



###  http://purl.org/cbv#installing

:installing rdf:type :BusinessStep ,
                     owl:NamedIndividual .



###  http://purl.org/cbv#inv

:inv rdf:type :TransactionType ,
              owl:NamedIndividual .



###  http://purl.org/cbv#killing

:killing rdf:type :BusinessStep ,
                  owl:NamedIndividual .



###  http://purl.org/cbv#loading

:loading rdf:type :BusinessStep ,
                  owl:NamedIndividual .



###  http://purl.org/cbv#non_sellable_damaged

:non_sellable_damaged rdf:type :Disposition ,
                               owl:NamedIndividual .



###  http://purl.org/cbv#non_sellable_disposed

:non_sellable_disposed rdf:type :Disposition ,
                                owl:NamedIndividual .



###  http://purl.org/cbv#non_sellable_expired

:non_sellable_expired rdf:type :Disposition ,
                               owl:NamedIndividual .



###  http://purl.org/cbv#non_sellable_no_pedigree_match

:non_sellable_no_pedigree_match rdf:type :Disposition ,
                                         owl:NamedIndividual .



###  http://purl.org/cbv#non_sellable_other

:non_sellable_other rdf:type :Disposition ,
                             owl:NamedIndividual .



###  http://purl.org/cbv#non_sellable_record

:non_sellable_record rdf:type :Disposition ,
                              owl:NamedIndividual .



###  http://purl.org/cbv#other

:other rdf:type :BusinessStep ,
                owl:NamedIndividual .



###  http://purl.org/cbv#owning_party

:owning_party rdf:type :SourceDestinationType ,
                       owl:NamedIndividual ;
              
              rdfs:comment """Added in CBV 1.1, The source or destination identifier denotes the party who owns (or is intended to own) the objects at the originating endpoint or
terminating endpoint (respectively) of the business transfer of which this EPCIS event is a part""" .



###  http://purl.org/cbv#packing

:packing rdf:type :BusinessStep ,
                  owl:NamedIndividual .



###  http://purl.org/cbv#pedigree

:pedigree rdf:type :TransactionType ,
                   owl:NamedIndividual .



###  http://purl.org/cbv#picking

:picking rdf:type :BusinessStep ,
                  owl:NamedIndividual .



###  http://purl.org/cbv#po

:po rdf:type :TransactionType ,
             owl:NamedIndividual .



###  http://purl.org/cbv#poc

:poc rdf:type :TransactionType ,
              owl:NamedIndividual .



###  http://purl.org/cbv#possessing_party

:possessing_party rdf:type :SourceDestinationType ,
                           owl:NamedIndividual ;
                  
                  rdfs:comment """The source or destination identifier denotes the party who
has (or is intended to have) physical possession of the
objects at the originating endpoint or terminating endpoint
(respectively) of the business transfer of which this EPCIS
event is a part.""" .



###  http://purl.org/cbv#production_order

:production_order rdf:type :TransactionType ,
                           owl:NamedIndividual ;
                  
                  rdfs:comment "Added in version 1.1" .



###  http://purl.org/cbv#recadv

:recadv rdf:type :TransactionType ,
                 owl:NamedIndividual .



###  http://purl.org/cbv#receiving

:receiving rdf:type :BusinessStep ,
                    owl:NamedIndividual .



###  http://purl.org/cbv#removing

:removing rdf:type :BusinessStep ,
                   owl:NamedIndividual .



###  http://purl.org/cbv#repacking

:repacking rdf:type :BusinessStep ,
                    owl:NamedIndividual .



###  http://purl.org/cbv#replacing

:replacing rdf:type :BusinessStep ,
                    owl:NamedIndividual .



###  http://purl.org/cbv#reserved

:reserved rdf:type :Disposition ,
                   owl:NamedIndividual .



###  http://purl.org/cbv#reserving

:reserving rdf:type :BusinessStep ,
                    owl:NamedIndividual .



###  http://purl.org/cbv#retail_selling

:retail_selling rdf:type :BusinessStep ,
                         owl:NamedIndividual .



###  http://purl.org/cbv#retail_sold

:retail_sold rdf:type :Disposition ,
                      owl:NamedIndividual .



###  http://purl.org/cbv#returned

:returned rdf:type :Disposition ,
                   owl:NamedIndividual .



###  http://purl.org/cbv#rma

:rma rdf:type :TransactionType ,
              owl:NamedIndividual .



###  http://purl.org/cbv#sellable_accesible

:sellable_accesible rdf:type :Disposition ,
                             owl:NamedIndividual .



###  http://purl.org/cbv#sellable_not_accessible

:sellable_not_accessible rdf:type :Disposition ,
                                  owl:NamedIndividual .



###  http://purl.org/cbv#shipping

:shipping rdf:type :BusinessStep ,
                   owl:NamedIndividual .



###  http://purl.org/cbv#stock_taking

:stock_taking rdf:type :BusinessStep ,
                       owl:NamedIndividual ;
              
              rdfs:comment "Added in version 1.1" .



###  http://purl.org/cbv#stocking

:stocking rdf:type :BusinessStep ,
                   owl:NamedIndividual .



###  http://purl.org/cbv#storing

:storing rdf:type :BusinessStep ,
                  owl:NamedIndividual .



###  http://purl.org/cbv#transforming

:transforming rdf:type :BusinessStep ,
                       owl:NamedIndividual .



###  http://purl.org/cbv#transporting

:transporting rdf:type :BusinessStep ,
                       owl:NamedIndividual ;
              
              rdfs:comment "Added in version 1.1" .



###  http://purl.org/cbv#unknown

:unknown rdf:type :Disposition ,
                  owl:NamedIndividual .



###  http://purl.org/cbv#unloading

:unloading rdf:type :BusinessStep ,
                    owl:NamedIndividual ;
           
           rdfs:comment "Added in version 1.1" .



###  http://purl.org/cbv#unpacking

:unpacking rdf:type :BusinessStep ,
                    owl:NamedIndividual ;
           
           rdfs:comment "Added in version 1.1" .




###  Generated by the OWL API (version 3.3.1957) http://owlapi.sourceforge.net

