<?xml version="1.0"?>


<!DOCTYPE rdf:RDF [
    <!ENTITY owl "http://www.w3.org/2002/07/owl#" >
    <!ENTITY dc "http://purl.org/dc/elements/1.1/" >
    <!ENTITY xsd "http://www.w3.org/2001/XMLSchema#" >
    <!ENTITY rdfs "http://www.w3.org/2000/01/rdf-schema#" >
    <!ENTITY rdf "http://www.w3.org/1999/02/22-rdf-syntax-ns#" >
]>


<rdf:RDF xmlns="http://purl.org/cbv#"
     xml:base="http://purl.org/cbv"
     xmlns:dc="http://purl.org/dc/elements/1.1/"
     xmlns:rdfs="http://www.w3.org/2000/01/rdf-schema#"
     xmlns:owl="http://www.w3.org/2002/07/owl#"
     xmlns:xsd="http://www.w3.org/2001/XMLSchema#"
     xmlns:rdf="http://www.w3.org/1999/02/22-rdf-syntax-ns#">
    <owl:Ontology rdf:about="http://purl.org/cbv">
        <owl:imports rdf:resource="http://protege.stanford.edu/plugins/owl/dc/protege-dc.owl"/>
    </owl:Ontology>
    


    <!-- 
    ///////////////////////////////////////////////////////////////////////////////////////
    //
    // Annotation properties
    //
    ///////////////////////////////////////////////////////////////////////////////////////
     -->

    <rdf:Description rdf:about="&dc;creator">
        <dc:creator>Monika Solanki(m.solanki@aston.ac.uk)</dc:creator>
    </rdf:Description>
    <rdf:Description rdf:about="&owl;versionInfo">
        <owl:versionInfo>1.1</owl:versionInfo>
    </rdf:Description>
    <owl:AnnotationProperty rdf:about="&rdfs;comment">
        <rdfs:comment>The CBVVocab is an OWL ontology that captures the identifiers in CBV 1.0 specification. (http://www.gs1.org/gsmp/kc/epcglobal/cbv/cbv_1_0-standard-20101013.pdf). The current version, CBVVocab 1.1, includes a partial set of the new identifiers to be included in CBV 1.1</rdfs:comment>
    </owl:AnnotationProperty>
    <rdf:Description rdf:about="&dc;title">
        <dc:title>CBVVocab 1.1</dc:title>
    </rdf:Description>
    


    <!-- 
    ///////////////////////////////////////////////////////////////////////////////////////
    //
    // Datatypes
    //
    ///////////////////////////////////////////////////////////////////////////////////////
     -->

    


    <!-- http://www.w3.org/1999/02/22-rdf-syntax-ns#PlainLiteral -->

    <rdfs:Datatype rdf:about="&rdf;PlainLiteral"/>
    


    <!-- http://www.w3.org/2000/01/rdf-schema#Literal -->

    <rdfs:Datatype rdf:about="&rdfs;Literal"/>
    


    <!-- http://www.w3.org/2001/XMLSchema#anyURI -->

    <rdfs:Datatype rdf:about="&xsd;anyURI"/>
    


    <!-- http://www.w3.org/2001/XMLSchema#positiveInteger -->

    <rdfs:Datatype rdf:about="&xsd;positiveInteger"/>
    


    <!-- http://www.w3.org/2001/XMLSchema#string -->

    <rdfs:Datatype rdf:about="&xsd;string"/>
    


    <!-- 
    ///////////////////////////////////////////////////////////////////////////////////////
    //
    // Object Properties
    //
    ///////////////////////////////////////////////////////////////////////////////////////
     -->

    


    <!-- http://purl.org/cbv#hasSite -->

    <owl:ObjectProperty rdf:about="http://purl.org/cbv#hasSite">
        <owl:inverseOf rdf:resource="http://purl.org/cbv#hasSubSite"/>
    </owl:ObjectProperty>
    


    <!-- http://purl.org/cbv#hasSubSite -->

    <owl:ObjectProperty rdf:about="http://purl.org/cbv#hasSubSite">
        <rdfs:domain rdf:resource="http://purl.org/cbv#Site"/>
        <rdfs:range rdf:resource="http://purl.org/cbv#SubSite"/>
    </owl:ObjectProperty>
    


    <!-- http://purl.org/cbv#hasSubSiteAttribute -->

    <owl:ObjectProperty rdf:about="http://purl.org/cbv#hasSubSiteAttribute"/>
    


    <!-- http://purl.org/cbv#hasSubSiteType -->

    <owl:ObjectProperty rdf:about="http://purl.org/cbv#hasSubSiteType"/>
    


    <!-- 
    ///////////////////////////////////////////////////////////////////////////////////////
    //
    // Data properties
    //
    ///////////////////////////////////////////////////////////////////////////////////////
     -->

    


    <!-- http://purl.org/cbv#hasLocationID -->

    <owl:DatatypeProperty rdf:about="http://purl.org/cbv#hasLocationID">
        <rdfs:domain rdf:resource="http://purl.org/cbv#Site"/>
        <rdfs:range rdf:resource="&xsd;string"/>
    </owl:DatatypeProperty>
    


    <!-- http://purl.org/cbv#hasNumericalCode -->

    <owl:DatatypeProperty rdf:about="http://purl.org/cbv#hasNumericalCode">
        <rdf:type rdf:resource="&owl;FunctionalProperty"/>
        <rdfs:domain rdf:resource="http://purl.org/cbv#SubSiteType"/>
        <rdfs:range rdf:resource="&xsd;positiveInteger"/>
    </owl:DatatypeProperty>
    


    <!-- http://purl.org/cbv#hasSubSiteDetail -->

    <owl:DatatypeProperty rdf:about="http://purl.org/cbv#hasSubSiteDetail">
        <owl:equivalentProperty rdf:resource="http://purl.org/cbv#ssd"/>
    </owl:DatatypeProperty>
    


    <!-- http://purl.org/cbv#ssd -->

    <owl:DatatypeProperty rdf:about="http://purl.org/cbv#ssd"/>
    


    <!-- 
    ///////////////////////////////////////////////////////////////////////////////////////
    //
    // Classes
    //
    ///////////////////////////////////////////////////////////////////////////////////////
     -->

    


    <!-- http://purl.org/cbv#BusinessStep -->

    <owl:Class rdf:about="http://purl.org/cbv#BusinessStep">
        <rdfs:comment> Denotes a specific activity within a business process. The business step field of an event specifies what business process step was taking place that caused the event to be captured. Example: an EPCIS event is generated as a product departs the location
identified by the Read Point. Business Step = &lt;The identifier that denotes“shipping”&gt;
</rdfs:comment>
    </owl:Class>
    


    <!-- http://purl.org/cbv#Disposition -->

    <owl:Class rdf:about="http://purl.org/cbv#Disposition">
        <rdfs:comment> Denotes the business state of an object. The disposition field of anevent specifies the business condition of the subject of the event (the things specified in the“what”
dimension), subsequent to the event. The disposition is assumed to hold true until another event indicates a change of disposition.  Example: an EPCIS event is generated and afterward the products can be sold as-is and customers can access product for purchase. Disposition = &lt;The identifier that denotes“sellable and accessible”&gt; </rdfs:comment>
    </owl:Class>
    


    <!-- http://purl.org/cbv#Site -->

    <owl:Class rdf:about="http://purl.org/cbv#Site">
        <owl:equivalentClass>
            <owl:Restriction>
                <owl:onProperty rdf:resource="http://purl.org/cbv#hasLocationID"/>
                <owl:qualifiedCardinality rdf:datatype="&xsd;nonNegativeInteger">1</owl:qualifiedCardinality>
                <owl:onDataRange rdf:resource="&xsd;string"/>
            </owl:Restriction>
        </owl:equivalentClass>
    </owl:Class>
    


    <!-- http://purl.org/cbv#SourceDestinationType -->

    <owl:Class rdf:about="http://purl.org/cbv#SourceDestinationType"/>
    


    <!-- http://purl.org/cbv#SubSite -->

    <owl:Class rdf:about="http://purl.org/cbv#SubSite">
        <owl:equivalentClass>
            <owl:Class>
                <owl:intersectionOf rdf:parseType="Collection">
                    <owl:Restriction>
                        <owl:onProperty rdf:resource="http://purl.org/cbv#hasSite"/>
                        <owl:someValuesFrom rdf:resource="http://purl.org/cbv#Site"/>
                    </owl:Restriction>
                    <owl:Restriction>
                        <owl:onProperty rdf:resource="http://purl.org/cbv#hasSubSiteType"/>
                        <owl:someValuesFrom rdf:resource="http://purl.org/cbv#SubSiteType"/>
                    </owl:Restriction>
                </owl:intersectionOf>
            </owl:Class>
        </owl:equivalentClass>
        <rdfs:subClassOf>
            <owl:Restriction>
                <owl:onProperty rdf:resource="http://purl.org/cbv#hasSubSiteAttribute"/>
                <owl:allValuesFrom rdf:resource="http://purl.org/cbv#SubSiteAttribute"/>
            </owl:Restriction>
        </rdfs:subClassOf>
        <rdfs:subClassOf>
            <owl:Restriction>
                <owl:onProperty rdf:resource="http://purl.org/cbv#hasSubSiteDetail"/>
                <owl:minCardinality rdf:datatype="&xsd;nonNegativeInteger">0</owl:minCardinality>
            </owl:Restriction>
        </rdfs:subClassOf>
        <rdfs:subClassOf>
            <owl:Restriction>
                <owl:onProperty rdf:resource="http://purl.org/cbv#hasSubSiteAttribute"/>
                <owl:minCardinality rdf:datatype="&xsd;nonNegativeInteger">0</owl:minCardinality>
            </owl:Restriction>
        </rdfs:subClassOf>
    </owl:Class>
    


    <!-- http://purl.org/cbv#SubSiteAttribute -->

    <owl:Class rdf:about="http://purl.org/cbv#SubSiteAttribute"/>
    


    <!-- http://purl.org/cbv#SubSiteType -->

    <owl:Class rdf:about="http://purl.org/cbv#SubSiteType"/>
    


    <!-- http://purl.org/cbv#TransactionType -->

    <owl:Class rdf:about="http://purl.org/cbv#TransactionType">
        <rdfs:comment> Denotes a particular kind of business transaction. Example: the identifier that denotes “purchase order”. </rdfs:comment>
    </owl:Class>
    


    <!-- http://www.w3.org/2002/07/owl#Thing -->

    <owl:Class rdf:about="&owl;Thing"/>
    


    <!-- 
    ///////////////////////////////////////////////////////////////////////////////////////
    //
    // Individuals
    //
    ///////////////////////////////////////////////////////////////////////////////////////
     -->

    


    <!-- http://purl.org/cbv#BackRoom -->

    <owl:NamedIndividual rdf:about="http://purl.org/cbv#BackRoom">
        <rdf:type rdf:resource="http://purl.org/cbv#SubSiteType"/>
        <hasNumericalCode rdf:datatype="&xsd;positiveInteger">201</hasNumericalCode>
        <rdfs:comment>An area within a store (all formats - club, etc) used to hold
product until it is purchased or can be moved to the sales floor</rdfs:comment>
    </owl:NamedIndividual>
    


    <!-- http://purl.org/cbv#CargoTerminal -->

    <owl:NamedIndividual rdf:about="http://purl.org/cbv#CargoTerminal">
        <rdf:type rdf:resource="http://purl.org/cbv#SubSiteType"/>
        <hasNumericalCode rdf:datatype="&xsd;positiveInteger">215</hasNumericalCode>
        <rdfs:comment>An area where cargo may get transferred between carriers.</rdfs:comment>
    </owl:NamedIndividual>
    


    <!-- http://purl.org/cbv#ColdStorage -->

    <owl:NamedIndividual rdf:about="http://purl.org/cbv#ColdStorage">
        <rdf:type rdf:resource="http://purl.org/cbv#SubSiteAttribute"/>
        <hasNumericalCode rdf:datatype="&xsd;positiveInteger">402</hasNumericalCode>
        <rdfs:comment>A specific area or room that maintains a temperature above
freezing but below ambient room temperature</rdfs:comment>
    </owl:NamedIndividual>
    


    <!-- http://purl.org/cbv#ContainerDeck -->

    <owl:NamedIndividual rdf:about="http://purl.org/cbv#ContainerDeck">
        <rdf:type rdf:resource="http://purl.org/cbv#SubSiteType"/>
        <hasNumericalCode rdf:datatype="&xsd;positiveInteger">214</hasNumericalCode>
        <rdfs:comment>An area on board a shipping vessel where containers are loaded.</rdfs:comment>
    </owl:NamedIndividual>
    


    <!-- http://purl.org/cbv#CustomerPickUpArea -->

    <owl:NamedIndividual rdf:about="http://purl.org/cbv#CustomerPickUpArea">
        <rdf:type rdf:resource="http://purl.org/cbv#SubSiteType"/>
        <hasNumericalCode rdf:datatype="&xsd;positiveInteger">212</hasNumericalCode>
        <rdfs:comment>An area designated at a store for customer to take possession of
purchased product.</rdfs:comment>
    </owl:NamedIndividual>
    


    <!-- http://purl.org/cbv#Electronics -->

    <owl:NamedIndividual rdf:about="http://purl.org/cbv#Electronics">
        <rdf:type rdf:resource="http://purl.org/cbv#SubSiteAttribute"/>
        <hasNumericalCode rdf:datatype="&xsd;positiveInteger">401</hasNumericalCode>
        <rdfs:comment>A specific area within the store for holding electronic products
such as TV&apos;s, DVD players, etc.</rdfs:comment>
    </owl:NamedIndividual>
    


    <!-- http://purl.org/cbv#Frozen -->

    <owl:NamedIndividual rdf:about="http://purl.org/cbv#Frozen">
        <rdf:type rdf:resource="http://purl.org/cbv#SubSiteAttribute"/>
        <hasNumericalCode rdf:datatype="&xsd;positiveInteger">402</hasNumericalCode>
        <rdfs:comment>A specific area or room that maintains a temperature at or below
freezing</rdfs:comment>
    </owl:NamedIndividual>
    


    <!-- http://purl.org/cbv#PackagingArea -->

    <owl:NamedIndividual rdf:about="http://purl.org/cbv#PackagingArea">
        <rdf:type rdf:resource="http://purl.org/cbv#SubSiteType"/>
        <hasNumericalCode rdf:datatype="&xsd;positiveInteger">251</hasNumericalCode>
        <rdfs:comment>An area within a facility where product is packaged.</rdfs:comment>
    </owl:NamedIndividual>
    


    <!-- http://purl.org/cbv#PharmacyArea -->

    <owl:NamedIndividual rdf:about="http://purl.org/cbv#PharmacyArea">
        <rdf:type rdf:resource="http://purl.org/cbv#SubSiteType"/>
        <hasNumericalCode rdf:datatype="&xsd;positiveInteger">253</hasNumericalCode>
    </owl:NamedIndividual>
    


    <!-- http://purl.org/cbv#PickingArea -->

    <owl:NamedIndividual rdf:about="http://purl.org/cbv#PickingArea">
        <rdf:type rdf:resource="http://purl.org/cbv#SubSiteType"/>
        <hasNumericalCode rdf:datatype="&xsd;positiveInteger">252</hasNumericalCode>
        <rdfs:comment>An area within a facility in which product is picked to fulfill an
order.</rdfs:comment>
    </owl:NamedIndividual>
    


    <!-- http://purl.org/cbv#ProductionArea -->

    <owl:NamedIndividual rdf:about="http://purl.org/cbv#ProductionArea">
        <rdf:type rdf:resource="http://purl.org/cbv#SubSiteType"/>
        <hasNumericalCode rdf:datatype="&xsd;positiveInteger">208</hasNumericalCode>
        <rdfs:comment>An area within a facility where the conversion of materials and
or assembly of components to manufacture goods, products or
services takes place.</rdfs:comment>
    </owl:NamedIndividual>
    


    <!-- http://purl.org/cbv#ReceivingArea -->

    <owl:NamedIndividual rdf:about="http://purl.org/cbv#ReceivingArea">
        <rdf:type rdf:resource="http://purl.org/cbv#SubSiteType"/>
        <hasNumericalCode rdf:datatype="&xsd;positiveInteger">209</hasNumericalCode>
        <rdfs:comment>An area within a facility where incoming merchandise is
unloaded and checked for condition and completeness</rdfs:comment>
    </owl:NamedIndividual>
    


    <!-- http://purl.org/cbv#ReturnsArea -->

    <owl:NamedIndividual rdf:about="http://purl.org/cbv#ReturnsArea">
        <rdf:type rdf:resource="http://purl.org/cbv#SubSiteType"/>
        <hasNumericalCode rdf:datatype="&xsd;positiveInteger">207</hasNumericalCode>
        <rdfs:comment>An area within a facility for holding or consolidating product to
be sent back to the supplier, shipper or designated location</rdfs:comment>
    </owl:NamedIndividual>
    


    <!-- http://purl.org/cbv#SalesFloor -->

    <owl:NamedIndividual rdf:about="http://purl.org/cbv#SalesFloor">
        <rdf:type rdf:resource="http://purl.org/cbv#SubSiteType"/>
        <hasNumericalCode rdf:datatype="&xsd;positiveInteger">203</hasNumericalCode>
        <rdfs:comment>An area within a store (all formats - club, etc) where product is
displayed for customer purchase</rdfs:comment>
    </owl:NamedIndividual>
    


    <!-- http://purl.org/cbv#SalesFloorTransitionArea -->

    <owl:NamedIndividual rdf:about="http://purl.org/cbv#SalesFloorTransitionArea">
        <rdf:type rdf:resource="http://purl.org/cbv#SubSiteType"/>
        <hasNumericalCode rdf:datatype="&xsd;positiveInteger">211</hasNumericalCode>
        <rdfs:comment>An area within a store between two physical locations (e.g.
Backroom and Sales Floor) - used for a read point only</rdfs:comment>
    </owl:NamedIndividual>
    


    <!-- http://purl.org/cbv#Shelf -->

    <owl:NamedIndividual rdf:about="http://purl.org/cbv#Shelf">
        <rdf:type rdf:resource="http://purl.org/cbv#SubSiteAttribute"/>
        <hasNumericalCode rdf:datatype="&xsd;positiveInteger">403</hasNumericalCode>
        <rdfs:comment>A specified internal location for holding product.</rdfs:comment>
    </owl:NamedIndividual>
    


    <!-- http://purl.org/cbv#ShippingArea -->

    <owl:NamedIndividual rdf:about="http://purl.org/cbv#ShippingArea">
        <rdf:type rdf:resource="http://purl.org/cbv#SubSiteType"/>
        <hasNumericalCode rdf:datatype="&xsd;positiveInteger">210</hasNumericalCode>
        <rdfs:comment>An area within a facility where outgoing merchandise is
checked for condition and completeness and loaded onto a
conveyance for transport</rdfs:comment>
    </owl:NamedIndividual>
    


    <!-- http://purl.org/cbv#StorageArea -->

    <owl:NamedIndividual rdf:about="http://purl.org/cbv#StorageArea">
        <rdf:type rdf:resource="http://purl.org/cbv#SubSiteType"/>
        <hasNumericalCode rdf:datatype="&xsd;positiveInteger">202</hasNumericalCode>
        <rdfs:comment>An area where product is kept within a facility to fulfill future
need.</rdfs:comment>
    </owl:NamedIndividual>
    


    <!-- http://purl.org/cbv#Undefined -->

    <owl:NamedIndividual rdf:about="http://purl.org/cbv#Undefined">
        <rdf:type rdf:resource="http://purl.org/cbv#SubSiteType"/>
        <hasNumericalCode rdf:datatype="&xsd;positiveInteger">299</hasNumericalCode>
        <rdfs:comment>Any sub-site type not identified by any of the listed values</rdfs:comment>
    </owl:NamedIndividual>
    


    <!-- http://purl.org/cbv#Yard -->

    <owl:NamedIndividual rdf:about="http://purl.org/cbv#Yard">
        <rdf:type rdf:resource="http://purl.org/cbv#SubSiteType"/>
        <hasNumericalCode rdf:datatype="&xsd;positiveInteger">213</hasNumericalCode>
        <rdfs:comment>An area outside of the main building used for holding product
(e.g. Trailer or container)</rdfs:comment>
    </owl:NamedIndividual>
    


    <!-- http://purl.org/cbv#accepting -->

    <owl:NamedIndividual rdf:about="http://purl.org/cbv#accepting">
        <rdf:type rdf:resource="http://purl.org/cbv#BusinessStep"/>
        <rdfs:comment>Denotes a specific activity within a business process where an object (i.e. product, shipment or asset) arrives into a location causing a change of 
        possession and/or responsibility.</rdfs:comment>
    </owl:NamedIndividual>
    


    <!-- http://purl.org/cbv#active -->

    <owl:NamedIndividual rdf:about="http://purl.org/cbv#active">
        <rdf:type rdf:resource="http://purl.org/cbv#Disposition"/>
    </owl:NamedIndividual>
    


    <!-- http://purl.org/cbv#arriving -->

    <owl:NamedIndividual rdf:about="http://purl.org/cbv#arriving">
        <rdf:type rdf:resource="http://purl.org/cbv#BusinessStep"/>
        <rdfs:comment>Shipment is arriving at a location</rdfs:comment>
    </owl:NamedIndividual>
    


    <!-- http://purl.org/cbv#assembling -->

    <owl:NamedIndividual rdf:about="http://purl.org/cbv#assembling">
        <rdf:type rdf:resource="http://purl.org/cbv#BusinessStep"/>
        <rdfs:comment>Denotes an activity within a business process whereby one or more trade item(s) or
        identifiable component parts are combined with other objects creating a new
        finished product. </rdfs:comment>
    </owl:NamedIndividual>
    


    <!-- http://purl.org/cbv#bol -->

    <owl:NamedIndividual rdf:about="http://purl.org/cbv#bol">
        <rdf:type rdf:resource="http://purl.org/cbv#TransactionType"/>
    </owl:NamedIndividual>
    


    <!-- http://purl.org/cbv#collecting -->

    <owl:NamedIndividual rdf:about="http://purl.org/cbv#collecting">
        <rdf:type rdf:resource="http://purl.org/cbv#BusinessStep"/>
        <rdfs:comment> Denotes a specific activity within a business process where an object (i.e.
        product, asset, shipment or container) is picked up and collected for future
        disposal, recycling or reused. </rdfs:comment>
    </owl:NamedIndividual>
    


    <!-- http://purl.org/cbv#commissioning -->

    <owl:NamedIndividual rdf:about="http://purl.org/cbv#commissioning">
        <rdf:type rdf:resource="http://purl.org/cbv#BusinessStep"/>
        <rdfs:comment>   Process of associating an EPC with a particular object (product, shipment, asset
        or container). A tag may have been encoded and applied in this step, or may have
        been previously encoded.  </rdfs:comment>
    </owl:NamedIndividual>
    


    <!-- http://purl.org/cbv#consigning -->

    <owl:NamedIndividual rdf:about="http://purl.org/cbv#consigning">
        <rdf:type rdf:resource="http://purl.org/cbv#BusinessStep"/>
        <rdfs:comment>Added in CBV 1.1. Indicates the overall process of staging_outbound, loading, departing, and accepting. 
It may be used when more granular process step
information is unknown or inaccessible. The use of consigning is
mutually exclusive from the use of staging_outbound, loading, departing, and accepting. 
Note: This business step is similar to shipping, but includes a change of possession and/or
ownership at the outbound side</rdfs:comment>
    </owl:NamedIndividual>
    


    <!-- http://purl.org/cbv#container__closed -->

    <owl:NamedIndividual rdf:about="http://purl.org/cbv#container__closed">
        <rdf:type rdf:resource="http://purl.org/cbv#Disposition"/>
    </owl:NamedIndividual>
    


    <!-- http://purl.org/cbv#cycle_counting -->

    <owl:NamedIndividual rdf:about="http://purl.org/cbv#cycle_counting">
        <rdf:type rdf:resource="http://purl.org/cbv#BusinessStep"/>
        <rdfs:comment>Added in version 1.1</rdfs:comment>
    </owl:NamedIndividual>
    


    <!-- http://purl.org/cbv#decommissioning -->

    <owl:NamedIndividual rdf:about="http://purl.org/cbv#decommissioning">
        <rdf:type rdf:resource="http://purl.org/cbv#BusinessStep"/>
        <rdfs:comment> Process of disassociating an EPC with an object (i.e. product, shipment, asset or container). EPC may
be re-commissioned at some point in the future and read again – however only with new
information. </rdfs:comment>
    </owl:NamedIndividual>
    


    <!-- http://purl.org/cbv#departing -->

    <owl:NamedIndividual rdf:about="http://purl.org/cbv#departing">
        <rdf:type rdf:resource="http://purl.org/cbv#BusinessStep"/>
        <rdfs:comment>   Shipment is leaving a location on its way to a destination </rdfs:comment>
    </owl:NamedIndividual>
    


    <!-- http://purl.org/cbv#desadv -->

    <owl:NamedIndividual rdf:about="http://purl.org/cbv#desadv">
        <rdf:type rdf:resource="http://purl.org/cbv#TransactionType"/>
    </owl:NamedIndividual>
    


    <!-- http://purl.org/cbv#destroyed -->

    <owl:NamedIndividual rdf:about="http://purl.org/cbv#destroyed">
        <rdf:type rdf:resource="http://purl.org/cbv#Disposition"/>
    </owl:NamedIndividual>
    


    <!-- http://purl.org/cbv#destroying -->

    <owl:NamedIndividual rdf:about="http://purl.org/cbv#destroying">
        <rdf:type rdf:resource="http://purl.org/cbv#BusinessStep"/>
        <rdfs:comment> Process of terminating an object (i.e. product, shipment, asset or shipping
        container) The object and its EPC should not be the subject of subsequent events
        that require a physical observation; subsequent physical observations are likely
        indicative of error (such as a stray read of a tag inside an incinerator)  </rdfs:comment>
    </owl:NamedIndividual>
    


    <!-- http://purl.org/cbv#disassembling -->

    <owl:NamedIndividual rdf:about="http://purl.org/cbv#disassembling">
        <rdf:type rdf:resource="http://purl.org/cbv#BusinessStep"/>
        <rdfs:comment>      Denotes a specific activity within a business process where a trade item is broken
        down into separate, uniquely identified component parts.  </rdfs:comment>
    </owl:NamedIndividual>
    


    <!-- http://purl.org/cbv#encoded -->

    <owl:NamedIndividual rdf:about="http://purl.org/cbv#encoded">
        <rdf:type rdf:resource="http://purl.org/cbv#Disposition"/>
    </owl:NamedIndividual>
    


    <!-- http://purl.org/cbv#encoding -->

    <owl:NamedIndividual rdf:about="http://purl.org/cbv#encoding">
        <rdf:type rdf:resource="http://purl.org/cbv#BusinessStep"/>
    </owl:NamedIndividual>
    


    <!-- http://purl.org/cbv#entering_exiting -->

    <owl:NamedIndividual rdf:about="http://purl.org/cbv#entering_exiting">
        <rdf:type rdf:resource="http://purl.org/cbv#BusinessStep"/>
    </owl:NamedIndividual>
    


    <!-- http://purl.org/cbv#holding -->

    <owl:NamedIndividual rdf:about="http://purl.org/cbv#holding">
        <rdf:type rdf:resource="http://purl.org/cbv#BusinessStep"/>
    </owl:NamedIndividual>
    


    <!-- http://purl.org/cbv#in_progress -->

    <owl:NamedIndividual rdf:about="http://purl.org/cbv#in_progress">
        <rdf:type rdf:resource="http://purl.org/cbv#Disposition"/>
    </owl:NamedIndividual>
    


    <!-- http://purl.org/cbv#in_transit -->

    <owl:NamedIndividual rdf:about="http://purl.org/cbv#in_transit">
        <rdf:type rdf:resource="http://purl.org/cbv#Disposition"/>
    </owl:NamedIndividual>
    


    <!-- http://purl.org/cbv#inactive -->

    <owl:NamedIndividual rdf:about="http://purl.org/cbv#inactive">
        <rdf:type rdf:resource="http://purl.org/cbv#Disposition"/>
    </owl:NamedIndividual>
    


    <!-- http://purl.org/cbv#inspecting -->

    <owl:NamedIndividual rdf:about="http://purl.org/cbv#inspecting">
        <rdf:type rdf:resource="http://purl.org/cbv#BusinessStep"/>
    </owl:NamedIndividual>
    


    <!-- http://purl.org/cbv#installing -->

    <owl:NamedIndividual rdf:about="http://purl.org/cbv#installing">
        <rdf:type rdf:resource="http://purl.org/cbv#BusinessStep"/>
    </owl:NamedIndividual>
    


    <!-- http://purl.org/cbv#inv -->

    <owl:NamedIndividual rdf:about="http://purl.org/cbv#inv">
        <rdf:type rdf:resource="http://purl.org/cbv#TransactionType"/>
    </owl:NamedIndividual>
    


    <!-- http://purl.org/cbv#killing -->

    <owl:NamedIndividual rdf:about="http://purl.org/cbv#killing">
        <rdf:type rdf:resource="http://purl.org/cbv#BusinessStep"/>
    </owl:NamedIndividual>
    


    <!-- http://purl.org/cbv#loading -->

    <owl:NamedIndividual rdf:about="http://purl.org/cbv#loading">
        <rdf:type rdf:resource="http://purl.org/cbv#BusinessStep"/>
    </owl:NamedIndividual>
    


    <!-- http://purl.org/cbv#non_sellable_damaged -->

    <owl:NamedIndividual rdf:about="http://purl.org/cbv#non_sellable_damaged">
        <rdf:type rdf:resource="http://purl.org/cbv#Disposition"/>
    </owl:NamedIndividual>
    


    <!-- http://purl.org/cbv#non_sellable_disposed -->

    <owl:NamedIndividual rdf:about="http://purl.org/cbv#non_sellable_disposed">
        <rdf:type rdf:resource="http://purl.org/cbv#Disposition"/>
    </owl:NamedIndividual>
    


    <!-- http://purl.org/cbv#non_sellable_expired -->

    <owl:NamedIndividual rdf:about="http://purl.org/cbv#non_sellable_expired">
        <rdf:type rdf:resource="http://purl.org/cbv#Disposition"/>
    </owl:NamedIndividual>
    


    <!-- http://purl.org/cbv#non_sellable_no_pedigree_match -->

    <owl:NamedIndividual rdf:about="http://purl.org/cbv#non_sellable_no_pedigree_match">
        <rdf:type rdf:resource="http://purl.org/cbv#Disposition"/>
    </owl:NamedIndividual>
    


    <!-- http://purl.org/cbv#non_sellable_other -->

    <owl:NamedIndividual rdf:about="http://purl.org/cbv#non_sellable_other">
        <rdf:type rdf:resource="http://purl.org/cbv#Disposition"/>
    </owl:NamedIndividual>
    


    <!-- http://purl.org/cbv#non_sellable_record -->

    <owl:NamedIndividual rdf:about="http://purl.org/cbv#non_sellable_record">
        <rdf:type rdf:resource="http://purl.org/cbv#Disposition"/>
    </owl:NamedIndividual>
    


    <!-- http://purl.org/cbv#other -->

    <owl:NamedIndividual rdf:about="http://purl.org/cbv#other">
        <rdf:type rdf:resource="http://purl.org/cbv#BusinessStep"/>
    </owl:NamedIndividual>
    


    <!-- http://purl.org/cbv#owning_party -->

    <owl:NamedIndividual rdf:about="http://purl.org/cbv#owning_party">
        <rdf:type rdf:resource="http://purl.org/cbv#SourceDestinationType"/>
        <rdfs:comment>Added in CBV 1.1, The source or destination identifier denotes the party who owns (or is intended to own) the objects at the originating endpoint or
terminating endpoint (respectively) of the business transfer of which this EPCIS event is a part</rdfs:comment>
    </owl:NamedIndividual>
    


    <!-- http://purl.org/cbv#packing -->

    <owl:NamedIndividual rdf:about="http://purl.org/cbv#packing">
        <rdf:type rdf:resource="http://purl.org/cbv#BusinessStep"/>
    </owl:NamedIndividual>
    


    <!-- http://purl.org/cbv#pedigree -->

    <owl:NamedIndividual rdf:about="http://purl.org/cbv#pedigree">
        <rdf:type rdf:resource="http://purl.org/cbv#TransactionType"/>
    </owl:NamedIndividual>
    


    <!-- http://purl.org/cbv#picking -->

    <owl:NamedIndividual rdf:about="http://purl.org/cbv#picking">
        <rdf:type rdf:resource="http://purl.org/cbv#BusinessStep"/>
    </owl:NamedIndividual>
    


    <!-- http://purl.org/cbv#po -->

    <owl:NamedIndividual rdf:about="http://purl.org/cbv#po">
        <rdf:type rdf:resource="http://purl.org/cbv#TransactionType"/>
    </owl:NamedIndividual>
    


    <!-- http://purl.org/cbv#poc -->

    <owl:NamedIndividual rdf:about="http://purl.org/cbv#poc">
        <rdf:type rdf:resource="http://purl.org/cbv#TransactionType"/>
    </owl:NamedIndividual>
    


    <!-- http://purl.org/cbv#possessing_party -->

    <owl:NamedIndividual rdf:about="http://purl.org/cbv#possessing_party">
        <rdf:type rdf:resource="http://purl.org/cbv#SourceDestinationType"/>
        <rdfs:comment>The source or destination identifier denotes the party who
has (or is intended to have) physical possession of the
objects at the originating endpoint or terminating endpoint
(respectively) of the business transfer of which this EPCIS
event is a part.</rdfs:comment>
    </owl:NamedIndividual>
    


    <!-- http://purl.org/cbv#production_order -->

    <owl:NamedIndividual rdf:about="http://purl.org/cbv#production_order">
        <rdf:type rdf:resource="http://purl.org/cbv#TransactionType"/>
        <rdfs:comment>Added in version 1.1</rdfs:comment>
    </owl:NamedIndividual>
    


    <!-- http://purl.org/cbv#recadv -->

    <owl:NamedIndividual rdf:about="http://purl.org/cbv#recadv">
        <rdf:type rdf:resource="http://purl.org/cbv#TransactionType"/>
    </owl:NamedIndividual>
    


    <!-- http://purl.org/cbv#receiving -->

    <owl:NamedIndividual rdf:about="http://purl.org/cbv#receiving">
        <rdf:type rdf:resource="http://purl.org/cbv#BusinessStep"/>
    </owl:NamedIndividual>
    


    <!-- http://purl.org/cbv#removing -->

    <owl:NamedIndividual rdf:about="http://purl.org/cbv#removing">
        <rdf:type rdf:resource="http://purl.org/cbv#BusinessStep"/>
    </owl:NamedIndividual>
    


    <!-- http://purl.org/cbv#repacking -->

    <owl:NamedIndividual rdf:about="http://purl.org/cbv#repacking">
        <rdf:type rdf:resource="http://purl.org/cbv#BusinessStep"/>
    </owl:NamedIndividual>
    


    <!-- http://purl.org/cbv#replacing -->

    <owl:NamedIndividual rdf:about="http://purl.org/cbv#replacing">
        <rdf:type rdf:resource="http://purl.org/cbv#BusinessStep"/>
    </owl:NamedIndividual>
    


    <!-- http://purl.org/cbv#reserved -->

    <owl:NamedIndividual rdf:about="http://purl.org/cbv#reserved">
        <rdf:type rdf:resource="http://purl.org/cbv#Disposition"/>
    </owl:NamedIndividual>
    


    <!-- http://purl.org/cbv#reserving -->

    <owl:NamedIndividual rdf:about="http://purl.org/cbv#reserving">
        <rdf:type rdf:resource="http://purl.org/cbv#BusinessStep"/>
    </owl:NamedIndividual>
    


    <!-- http://purl.org/cbv#retail_selling -->

    <owl:NamedIndividual rdf:about="http://purl.org/cbv#retail_selling">
        <rdf:type rdf:resource="http://purl.org/cbv#BusinessStep"/>
    </owl:NamedIndividual>
    


    <!-- http://purl.org/cbv#retail_sold -->

    <owl:NamedIndividual rdf:about="http://purl.org/cbv#retail_sold">
        <rdf:type rdf:resource="http://purl.org/cbv#Disposition"/>
    </owl:NamedIndividual>
    


    <!-- http://purl.org/cbv#returned -->

    <owl:NamedIndividual rdf:about="http://purl.org/cbv#returned">
        <rdf:type rdf:resource="http://purl.org/cbv#Disposition"/>
    </owl:NamedIndividual>
    


    <!-- http://purl.org/cbv#rma -->

    <owl:NamedIndividual rdf:about="http://purl.org/cbv#rma">
        <rdf:type rdf:resource="http://purl.org/cbv#TransactionType"/>
    </owl:NamedIndividual>
    


    <!-- http://purl.org/cbv#sellable_accesible -->

    <owl:NamedIndividual rdf:about="http://purl.org/cbv#sellable_accesible">
        <rdf:type rdf:resource="http://purl.org/cbv#Disposition"/>
    </owl:NamedIndividual>
    


    <!-- http://purl.org/cbv#sellable_not_accessible -->

    <owl:NamedIndividual rdf:about="http://purl.org/cbv#sellable_not_accessible">
        <rdf:type rdf:resource="http://purl.org/cbv#Disposition"/>
    </owl:NamedIndividual>
    


    <!-- http://purl.org/cbv#shipping -->

    <owl:NamedIndividual rdf:about="http://purl.org/cbv#shipping">
        <rdf:type rdf:resource="http://purl.org/cbv#BusinessStep"/>
    </owl:NamedIndividual>
    


    <!-- http://purl.org/cbv#stock_taking -->

    <owl:NamedIndividual rdf:about="http://purl.org/cbv#stock_taking">
        <rdf:type rdf:resource="http://purl.org/cbv#BusinessStep"/>
        <rdfs:comment>Added in version 1.1</rdfs:comment>
    </owl:NamedIndividual>
    


    <!-- http://purl.org/cbv#stocking -->

    <owl:NamedIndividual rdf:about="http://purl.org/cbv#stocking">
        <rdf:type rdf:resource="http://purl.org/cbv#BusinessStep"/>
    </owl:NamedIndividual>
    


    <!-- http://purl.org/cbv#storing -->

    <owl:NamedIndividual rdf:about="http://purl.org/cbv#storing">
        <rdf:type rdf:resource="http://purl.org/cbv#BusinessStep"/>
    </owl:NamedIndividual>
    


    <!-- http://purl.org/cbv#transforming -->

    <owl:NamedIndividual rdf:about="http://purl.org/cbv#transforming">
        <rdf:type rdf:resource="http://purl.org/cbv#BusinessStep"/>
    </owl:NamedIndividual>
    


    <!-- http://purl.org/cbv#transporting -->

    <owl:NamedIndividual rdf:about="http://purl.org/cbv#transporting">
        <rdf:type rdf:resource="http://purl.org/cbv#BusinessStep"/>
        <rdfs:comment>Added in version 1.1</rdfs:comment>
    </owl:NamedIndividual>
    


    <!-- http://purl.org/cbv#unknown -->

    <owl:NamedIndividual rdf:about="http://purl.org/cbv#unknown">
        <rdf:type rdf:resource="http://purl.org/cbv#Disposition"/>
    </owl:NamedIndividual>
    


    <!-- http://purl.org/cbv#unloading -->

    <owl:NamedIndividual rdf:about="http://purl.org/cbv#unloading">
        <rdf:type rdf:resource="http://purl.org/cbv#BusinessStep"/>
        <rdfs:comment>Added in version 1.1</rdfs:comment>
    </owl:NamedIndividual>
    


    <!-- http://purl.org/cbv#unpacking -->

    <owl:NamedIndividual rdf:about="http://purl.org/cbv#unpacking">
        <rdf:type rdf:resource="http://purl.org/cbv#BusinessStep"/>
        <rdfs:comment>Added in version 1.1</rdfs:comment>
    </owl:NamedIndividual>
</rdf:RDF>



<!-- Generated by the OWL API (version 3.3.1957) http://owlapi.sourceforge.net -->

