@prefix : <https://w3id.org/dio#> .
@prefix dc: <http://purl.org/dc/elements/1.1/> .
@prefix dio: <https://w3id.org/dio#> .
@prefix owl: <http://www.w3.org/2002/07/owl#> .
@prefix rdf: <http://www.w3.org/1999/02/22-rdf-syntax-ns#> .
@prefix xml: <http://www.w3.org/XML/1998/namespace> .
@prefix xsd: <http://www.w3.org/2001/XMLSchema#> .
@prefix rdfs: <http://www.w3.org/2000/01/rdf-schema#> .
@base <https://w3id.org/dio#> .

<https://w3id.org/dio#> rdf:type owl:Ontology ;
                         dc:creator "Monika Solanki (monika.solanki@cs.ox.ac.uk)"@en ;
                         dc:date "04-01-2016" ;
                         dc:description """The Design Intent Ontology (DIO) is a generic ontology that provides the conceptualisation needed to capture the knowledge generated during various phases of the overall design lifecycle. 

It provides definitions for design artifacts such as requirements, designs, design issues, solutions, justifications and evidence and relationships between them to represent the design process and how these things lead to design outcomes.  It draws upon the paradigms of IBIS(Interactive Intent-Based Illustration), argumentation and design rationale. It is linked to W3C PROV by defining the actors in the design process as PROV agents and the design artifacts themselves are PROV entities. However DIO uses a modualrised version of PROV-O, based on Syntactic locality.

DIO makes few assumptions about the design process used as the definitions of these activities properly belongs in the software lifecycle and data lifecycle models. The Figure below illustrates the conceptual entities in DIO and their relationships."""^^xsd:string ;
                         dc:title "The Design Intent Ontology - A content ontology design pattern" ;
                         rdfs:seeAlso "http://ceur-ws.org/Vol-1461/WOP2015_pattern_abstract_6.pdf"^^xsd:anyURI ;
                         owl:versionInfo "1.1.000"^^xsd:string .

#################################################################
#    Object Properties
#################################################################

###  https://w3id.org/dio#addressedBy
dio:addressedBy rdf:type owl:ObjectProperty ;
                rdfs:comment "A relationship stating the design intent addressing a requirement." ;
                rdfs:label "addressedBy" .


###  https://w3id.org/dio#captureMethodology
dio:captureMethodology rdf:type owl:ObjectProperty ;
                       rdfs:comment "A relationship identifying the capture methodology for a design issue" ;
                       rdfs:label "captureMethodology" .


###  https://w3id.org/dio#contradicts
dio:contradicts rdf:type owl:ObjectProperty ;
                rdfs:domain dio:Solution ;
                rdfs:range dio:Solution ;
                rdfs:comment "A relationship indicating contradictory issues." ;
                rdfs:label "contradicts" .


###  https://w3id.org/dio#fulfillsRequirement
dio:fulfillsRequirement rdf:type owl:ObjectProperty ;
                        owl:inverseOf dio:requirementFulfilledBy ;
                        rdfs:domain dio:Design ,
                                    dio:DesignIntentArtifact ;
                        rdfs:range dio:DesignRequirement ;
                        rdfs:comment "A relationship between the design and its requirement." ;
                        rdfs:label "fullfillsRequirements" .


###  https://w3id.org/dio#generatedByIntent
dio:generatedByIntent rdf:type owl:ObjectProperty ;
                      owl:inverseOf dio:generatesIssue ;
                      rdfs:comment "A relationship between the design issue and intent." ;
                      rdfs:label "generatedByIntent" .


###  https://w3id.org/dio#generatesIssue
dio:generatesIssue rdf:type owl:ObjectProperty ;
                   rdfs:comment "A relationship between the design intent and issue." ;
                   rdfs:label "generatesIssue" .


###  https://w3id.org/dio#governsDesign
dio:governsDesign rdf:type owl:ObjectProperty ;
                  rdfs:domain dio:DesignDecision ;
                  rdfs:range dio:Design ;
                  rdfs:comment "The design decision governing the design." ;
                  rdfs:label "governsDesign" .


###  https://w3id.org/dio#hasAlternativeSolution
dio:hasAlternativeSolution rdf:type owl:ObjectProperty ;
                           rdfs:subPropertyOf owl:topObjectProperty ;
                           owl:inverseOf dio:providesAlternativeSolution ;
                           rdfs:range dio:AlternativeSolution ;
                           rdfs:comment "The realtionship between the issue and an alternative solution for it." ;
                           rdfs:label "hasAlternativeSolution" .


###  https://w3id.org/dio#hasArgument
dio:hasArgument rdf:type owl:ObjectProperty ;
                rdfs:range dio:Argument ;
                rdfs:comment "The relationship between a solution and an argument made against it." ;
                rdfs:label "hasArgument" .


###  https://w3id.org/dio#hasComment
dio:hasComment rdf:type owl:ObjectProperty ;
               rdfs:comment "The relationship between a comment and a design intent artifact for which the comment is made." ;
               rdfs:label "hasComment" .


###  https://w3id.org/dio#hasConstraint
dio:hasConstraint rdf:type owl:ObjectProperty ;
                  rdfs:domain dio:Solution ;
                  rdfs:range dio:Constraint ;
                  rdfs:comment "A relationship between a solution and a constarint on it." ;
                  rdfs:label "hasConstraint" .


###  https://w3id.org/dio#hasEvidence
dio:hasEvidence rdf:type owl:ObjectProperty ;
                rdfs:domain dio:Argument ,
                            dio:Justification ;
                rdfs:range dio:Evidence ;
                rdfs:comment "A relationship between a solution and an evidence for it." ;
                rdfs:label "hasEvidence" .


###  https://w3id.org/dio#hasJustification
dio:hasJustification rdf:type owl:ObjectProperty ;
                     rdfs:range dio:Justification ;
                     rdfs:comment "A relationship between a solution and the justification for it." ;
                     rdfs:label "hasJustification" .


###  https://w3id.org/dio#hasMandatedSolution
dio:hasMandatedSolution rdf:type owl:ObjectProperty ;
                        rdfs:subPropertyOf owl:topObjectProperty ;
                        owl:inverseOf dio:providesMandatedSolution ;
                        rdfs:range dio:MandatedSolution ;
                        rdfs:comment "A relationship between the issue and its mandated solution." ;
                        rdfs:label "hasMandatedSolution" .


###  https://w3id.org/dio#hasStatus
dio:hasStatus rdf:type owl:ObjectProperty ;
              rdfs:domain dio:DesignIssue ;
              rdfs:range dio:Status ;
              rdfs:comment "The relationship between an issue and its status." ;
              rdfs:label "hasStatus" .


###  https://w3id.org/dio#identifiedByRequirement
dio:identifiedByRequirement rdf:type owl:ObjectProperty ;
                            owl:inverseOf dio:identifies ;
                            rdfs:comment "The relationship between an issue and the requirement that identifies it." ;
                            rdfs:label "identifiedByRequirement" .


###  https://w3id.org/dio#identifies
dio:identifies rdf:type owl:ObjectProperty ;
               rdfs:comment "A relationship between the requirement and the issue it identifies." .


###  https://w3id.org/dio#implementedBy
dio:implementedBy rdf:type owl:ObjectProperty .


###  https://w3id.org/dio#leadsTo
dio:leadsTo rdf:type owl:ObjectProperty ;
            rdfs:subPropertyOf owl:topObjectProperty ;
            rdfs:domain dio:MandatedSolution ;
            rdfs:range dio:DesignDecision ;
            rdfs:comment "A relationship between a mandated solution and design decision made based on it." ;
            rdfs:label "leadsTo" .


###  https://w3id.org/dio#providesAlternativeSolution
dio:providesAlternativeSolution rdf:type owl:ObjectProperty ;
                                rdfs:comment "A relationship between an alternative solution and the issue." ;
                                rdfs:label "providesAlternativeSolution" .


###  https://w3id.org/dio#providesMandatedSolution
dio:providesMandatedSolution rdf:type owl:ObjectProperty ;
                             rdfs:comment "A relationship between a mandated solution and the issue." ;
                             rdfs:label "providesMandatedSolution" .


###  https://w3id.org/dio#rationaleCapturedUsing
dio:rationaleCapturedUsing rdf:type owl:ObjectProperty ;
                           rdfs:comment "A relationship between the design rationale and its capture methodology." ;
                           rdfs:label "rationaleCapturedUsing" .


###  https://w3id.org/dio#refines
dio:refines rdf:type owl:ObjectProperty ;
            rdfs:domain dio:Solution ;
            rdfs:range dio:Solution ;
            rdfs:comment "A relationship between two requirememts when one refines the other." ;
            rdfs:label "refines" .


###  https://w3id.org/dio#requirementFulfilledBy
dio:requirementFulfilledBy rdf:type owl:ObjectProperty ;
                           rdfs:comment "A relationship between the design and its originating requirements" ;
                           rdfs:label "requirementFulfilledBy" .


###  https://w3id.org/dio#supports
dio:supports rdf:type owl:ObjectProperty ;
             rdfs:range dio:Argument ,
                        dio:Justification ;
             rdfs:comment "A relationship between an agent and a design solution argument or justification." ;
             rdfs:label "supports" .


###  https://w3id.org/dio#usesAssumption
dio:usesAssumption rdf:type owl:ObjectProperty ;
                   rdfs:domain dio:Solution ;
                   rdfs:range dio:Assumption ;
                   rdfs:comment "A relationship between a solution and the Assumption it makes." ;
                   rdfs:label "usesAssumption" .


###  https://w3id.org/dio#usesHeuristic
dio:usesHeuristic rdf:type owl:ObjectProperty ;
                  rdfs:domain dio:Solution ;
                  rdfs:range dio:Heuristic ;
                  rdfs:comment "A relationship between a solution and the heuristic iy uses." ;
                  rdfs:label "usesHeuristic" .


#################################################################
#    Data properties
#################################################################

###  http://www.w3.org/ns/prov#generatedAtTime
<http://www.w3.org/ns/prov#generatedAtTime> rdf:type owl:DatatypeProperty .


###  https://w3id.org/dio#version
dio:version rdf:type owl:DatatypeProperty ,
                     owl:FunctionalProperty .


#################################################################
#    Classes
#################################################################

###  http://www.w3.org/ns/prov#Agent
<http://www.w3.org/ns/prov#Agent> rdf:type owl:Class .


###  https://w3id.org/dio#AlternativeSolution
dio:AlternativeSolution rdf:type owl:Class ;
                        rdfs:subClassOf dio:Solution ;
                        rdfs:comment "An entity representing the proposed solution." ;
                        rdfs:label "Alternative Solution" .


###  https://w3id.org/dio#Argument
dio:Argument rdf:type owl:Class ;
             rdfs:subClassOf dio:DesignIntentArtifact ;
             rdfs:comment "A reason presented against a proposed solution." ;
             rdfs:label "Argument" .


###  https://w3id.org/dio#Assumption
dio:Assumption rdf:type owl:Class ;
               rdfs:subClassOf dio:DesignIntentArtifact ;
               rdfs:comment "The assumption on which a proposed solution is based." ;
               rdfs:label "Assumption" .


###  https://w3id.org/dio#Comment
dio:Comment rdf:type owl:Class ;
            rdfs:subClassOf dio:DesignIntentArtifact ;
            rdfs:comment "A comment made by an agent in response to an argument, a justification or another comment" ;
            rdfs:label "Comment" .


###  https://w3id.org/dio#Constraint
dio:Constraint rdf:type owl:Class ;
               rdfs:subClassOf dio:DesignIntentArtifact ;
               rdfs:comment "A constraint that underlies the proposed solution." ;
               rdfs:label "Constraint" .


###  https://w3id.org/dio#Design
dio:Design rdf:type owl:Class ;
           rdfs:comment "A design is a specification of an object, manifested by an agent, intended to accomplish goals, in a particular environment, using a set of  components, satisfying a set of requirements, subject to constraints." ;
           rdfs:label "Design" .


###  https://w3id.org/dio#DesignArtifact
dio:DesignArtifact rdf:type owl:Class ;
                   rdfs:comment "The concrete artifact that is implemented or developed following the design that emerges from the design decisions." ;
                   rdfs:label "Design Artifact" .


###  https://w3id.org/dio#DesignDecision
dio:DesignDecision rdf:type owl:Class ;
                   rdfs:comment "The final design decision made based on the various alternative solutions proposed. A design decision is driven by a mandated solution." ;
                   rdfs:label "Design Decision" .


###  https://w3id.org/dio#DesignGoal
dio:DesignGoal rdf:type owl:Class ;
               owl:equivalentClass dio:DesignIssue ;
               rdfs:subClassOf [ owl:intersectionOf ( dio:DesignIntentArtifact
                                                      [ rdf:type owl:Restriction ;
                                                        owl:onProperty dio:hasAlternativeSolution ;
                                                        owl:allValuesFrom dio:AlternativeSolution
                                                      ]
                                                      [ rdf:type owl:Restriction ;
                                                        owl:onProperty dio:hasMandatedSolution ;
                                                        owl:allValuesFrom dio:MandatedSolution
                                                      ]
                                                      [ rdf:type owl:Restriction ;
                                                        owl:onProperty dio:hasMandatedSolution ;
                                                        owl:maxQualifiedCardinality "1"^^xsd:nonNegativeInteger ;
                                                        owl:onClass dio:MandatedSolution
                                                      ]
                                                    ) ;
                                 rdf:type owl:Class
                               ] ;
               rdfs:comment "An entity representing the problem, goal, question or issue the design intent aims to address." ;
               rdfs:label "Design Goal" .


###  https://w3id.org/dio#DesignIntent
dio:DesignIntent rdf:type owl:Class ;
                 rdfs:subClassOf dio:DesignIntentArtifact ;
                 rdfs:comment "A entity defining the notion of a design intent, i.e., the rationale underpinning the choices that are made from the alternatives available during various phases of the overall design lifecycle." ;
                 rdfs:label "Design Intent" .


###  https://w3id.org/dio#DesignIntentArtifact
dio:DesignIntentArtifact rdf:type owl:Class ;
                         rdfs:subClassOf [ owl:intersectionOf ( [ rdf:type owl:Restriction ;
                                                                  owl:onProperty <http://www.w3.org/ns/prov#wasAttributedTo> ;
                                                                  owl:qualifiedCardinality "1"^^xsd:nonNegativeInteger ;
                                                                  owl:onClass <http://www.w3.org/ns/prov#Agent>
                                                                ]
                                                                [ rdf:type owl:Restriction ;
                                                                  owl:onProperty <http://www.w3.org/ns/prov#generatedAtTime> ;
                                                                  owl:qualifiedCardinality "1"^^xsd:nonNegativeInteger ;
                                                                  owl:onDataRange xsd:dateTime
                                                                ]
                                                                [ rdf:type owl:Restriction ;
                                                                  owl:onProperty dio:version ;
                                                                  owl:qualifiedCardinality "1"^^xsd:nonNegativeInteger ;
                                                                  owl:onDataRange xsd:string
                                                                ]
                                                              ) ;
                                           rdf:type owl:Class
                                         ] ;
                         rdfs:comment "An entity representing any artifact that plays a part in capturing the design intent. The minimum ontological commitment required for this entity is a brief description of the artifact, the version info and the date." ;
                         rdfs:label "Design Intent Artifact" .


###  https://w3id.org/dio#DesignIssue
dio:DesignIssue rdf:type owl:Class ;
                rdfs:subClassOf dio:DesignIntentArtifact ;
                rdfs:comment "An entity representing the problem, goal, question or issue the design intent aims to address." ;
                rdfs:label "Design Issue" .


###  https://w3id.org/dio#DesignRequirement
dio:DesignRequirement rdf:type owl:Class ;
                      rdfs:subClassOf dio:DesignIntentArtifact ;
                      rdfs:comment "An entity capturing the requirements that result in the design intent" ;
                      rdfs:label "Design Requirements" .


###  https://w3id.org/dio#Evaluation
dio:Evaluation rdf:type owl:Class ;
               rdfs:subClassOf dio:DesignIntentArtifact ;
               rdfs:comment "An entity representing the evaluation that supports the solution." ;
               rdfs:label "Evaluation" .


###  https://w3id.org/dio#Evidence
dio:Evidence rdf:type owl:Class ;
             rdfs:subClassOf dio:DesignIntentArtifact ;
             rdfs:comment "An entity representing an evidence that supports a proposed solution." ;
             rdfs:label "Evidence" .


###  https://w3id.org/dio#Heuristic
dio:Heuristic rdf:type owl:Class ;
              rdfs:subClassOf dio:DesignIntentArtifact ;
              rdfs:comment "An entity representing the requirements to be fulfilled for realising the solution" ;
              rdfs:label "Heuristic" .


###  https://w3id.org/dio#Justification
dio:Justification rdf:type owl:Class ;
                  rdfs:subClassOf dio:DesignIntentArtifact ;
                  rdfs:comment "A reason supporting the proposed solution." ;
                  rdfs:label "Justification" .


###  https://w3id.org/dio#MandatedSolution
dio:MandatedSolution rdf:type owl:Class ;
                     rdfs:subClassOf dio:Solution ;
                     rdfs:comment "An entity representing the solution accepted as a result of the design deliberation process." ;
                     rdfs:label "Mandated Solution" .


###  https://w3id.org/dio#RationaleCaptureMethod
dio:RationaleCaptureMethod rdf:type owl:Class ;
                           rdfs:comment "An entity representing the methodology used to capture the design intent artifact" ;
                           rdfs:label "Rationale Capture Methodology" .


###  https://w3id.org/dio#Solution
dio:Solution rdf:type owl:Class ;
             rdfs:subClassOf dio:DesignIntentArtifact ;
             rdfs:label "Solution" .


###  https://w3id.org/dio#Status
dio:Status rdf:type owl:Class ;
           rdfs:comment "An entity representing the status of a design issue." ;
           rdfs:label "Status" .


#################################################################
#    Individuals
#################################################################

###  https://w3id.org/dio#Active
dio:Active rdf:type owl:NamedIndividual ,
                    dio:Status ;
           rdfs:comment "The status of an issue when it is active." ;
           rdfs:label "Active" .


###  https://w3id.org/dio#OnHold
dio:OnHold rdf:type owl:NamedIndividual ,
                    dio:Status ;
           rdfs:comment "The status of an issue when it is onHold" ;
           rdfs:label "onHold" .


###  https://w3id.org/dio#Resolved
dio:Resolved rdf:type owl:NamedIndividual ,
                      dio:Status ;
             rdfs:comment "The status of an issue when it is resolved." .


###  https://w3id.org/dio#Terminated
dio:Terminated rdf:type owl:NamedIndividual ,
                        dio:Status ;
               rdfs:comment "The status of an issue when it is terminated." .


###  Generated by the OWL API (version 4.5.9.2019-02-01T07:24:44Z) https://github.com/owlcs/owlapi
